Added reduction from mu_halting to lambda calculus

theories/L/Computability/Synthetic.v
@@ -14,6 +14,9 @@ Definition L_enumerable {X} `{registered X} (p : X -> Prop) :=
   exists f : nat -> option X, is_computable f /\ (enumerates f p).
 
 Definition L_recognisable {X} `{registered X} (p : X -> Prop) :=
+  exists f : X -> nat -> bool, is_computable f /\ forall x, p x <-> exists n, f x n = true.
+
+Definition L_recognisable' {X} `{registered X} (p : X -> Prop) :=
   exists s : term, forall x, p x <-> converges (s (enc x)).
 
 Section L_enum_rec.
@@ -39,7 +42,7 @@ Section L_enum_rec.
   Qed.
     
   Lemma L_enumerable_recognisable :
-    L_recognisable p.
+    L_recognisable' p.
   Proof.
     exists (λ x, !!mu (λ y, !!(ext test) x y)).
     intros. split; intros.
@@ -156,3 +159,24 @@ Proof.
   - now exists (fun x0 => x (enc x0)). 
 Qed.  
 
+Lemma L_recognisable'_recognisable {X} `{registered X} (p : X -> Prop) :
+  L_recognisable p -> L_recognisable' p.
+Proof.
+  intros (f & [c_f] & H_f).
+  exists (lam (mu (lam (ext f 1 0)))).
+  intros. 
+  assert (((lam (mu (lam ((ext f 1) 0)))) (enc x)) >* mu (lam (ext f (enc x) 0))) by Lsimpl.
+  rewrite H0. rewrite mu_spec.
+  - rewrite H_f. split; intros [n]; exists n.
+    Lsimpl. now rewrite H1.
+    eapply enc_extinj.
+    now assert ((lam (((ext f) (enc x)) 0)) (ext n) == enc (f x n)) as <- by Lsimpl.
+  - Lproc.
+  - intros. exists (f x n). Lsimpl.
+Qed.    
+
+Lemma L_recognisable_halt {X} `{registered X} (p : X -> Prop) :
+  L_recognisable p -> p ⪯ converges.
+Proof.
+  intros. eapply L_recognisable'_recognisable in H0 as  (f & H_f). now exists (fun x0 => f (enc x0)). 
+Qed.
