theories/L/Reductions/MuRec.v
@@ -1,94 +1,48 @@
 From Undecidability.H10 Require Import H10 dio_single dio_logic.
 From Undecidability.L.Datatypes Require Import LNat Lists LOptions LSum.
 From Undecidability.L Require Import Tactics.LTactics Computability.MuRec Computability.Synthetic Tactics.GenEncode.
-
-
-
-(**************************************************************)
-(*   Copyright Dominique Larchey-Wendling [*]                 *)
-(*                                                            *)
-(*                             [*] Affiliation LORIA -- CNRS  *)
-(**************************************************************)
-(*      This file is distributed under the terms of the       *)
-(*         CeCILL v2 FREE SOFTWARE LICENSE AGREEMENT          *)
-(**************************************************************)
-
 From Undecidability.Shared Require Import DLW.Vec.vec DLW.Vec.pos.
-From Undecidability.MuRec Require Import recalg.
+From Undecidability.MuRec Require Import recalg ra_bs ra_sem_eq.
 
-Set Implicit Arguments.
-
-Reserved Notation "  '[' f ';' v ']' '~~>' x " (at level 70).
+Reserved Notation "  '[' f ';' v ';' min ';' c ']' '~~>' x " (at level 70).
 
 (* Bigstep semantics for recursive algorithms *)
    
-Inductive ra_bs : forall k, recalg k -> vec nat k -> nat -> Prop :=
-    | in_ra_bs_cst  : forall n v,             [ra_cst n;        v] ~~> n
-    | in_ra_bs_zero : forall v,               [ra_zero;         v] ~~> 0
-    | in_ra_bs_succ : forall v,               [ra_succ;         v] ~~> S (vec_head v)
-    | in_ra_bs_proj : forall k v j,           [@ra_proj k j;    v] ~~> vec_pos v j
+Inductive ra_bs_c : nat -> nat -> forall k, recalg k -> vec nat k -> nat -> Prop := 
+    | in_ra_bs_c_cst  : forall min c n v,             [ra_cst n;        v; min; S c] ~~> n
+    | in_ra_bs_c_zero : forall min c v,               [ra_zero;         v; min; S c] ~~> 0
+    | in_ra_bs_c_succ : forall min c v,               [ra_succ;         v; min; S c] ~~> S (vec_head v)
+    | in_ra_bs_c_proj : forall min c k v j,           [@ra_proj k j;    v; min; S c] ~~> vec_pos v j 
     
-    | in_ra_bs_comp : forall k i f (gj : vec (recalg i) k) v w x,
-                                   (forall j, [vec_pos gj j;    v] ~~> vec_pos w j)
-                               ->             [f;               w] ~~> x
-                               ->             [ra_comp f gj;    v] ~~> x
+    | in_ra_bs_c_comp : forall min c k i f (gj : vec (recalg i) k) v w x,
+                                         (forall j, [vec_pos gj j;    v; min; c - pos2nat j] ~~> vec_pos w j)
+                                 ->             [f;               w; min; S c] ~~> x
+                                 ->             [ra_comp f gj;    v; min; S (S c)] ~~> x
 
-    | in_ra_bs_rec_0 : forall k f (g : recalg (S (S k))) v x,
-                                              [f;               v] ~~> x
-                               ->             [ra_rec f g;   0##v] ~~> x
+    | in_ra_bs_c_rec_0 : forall min c k f (g : recalg (S (S k))) v x,    
+                                               [f;               v; min; c] ~~> x 
+                                 ->             [ra_rec f g;   0##v; min; S c] ~~> x
 
-    | in_ra_bs_rec_S : forall k f (g : recalg (S (S k))) v n x y,
-                                              [ra_rec f g;   n##v] ~~> x
-                               ->             [g;         n##x##v] ~~> y
-                               ->             [ra_rec f g; S n##v] ~~> y
+    | in_ra_bs_c_rec_S : forall min c k f (g : recalg (S (S k))) v n x y,          
+                                             [ra_rec f g;   n##v; min; c] ~~> x
+                               ->             [g;         n##x##v; min; c] ~~> y
+                               ->             [ra_rec f g; S n##v; min; S c] ~~> y
                                
-    | in_ra_bs_min : forall k (f : recalg (S k)) v x w ,
-                           (forall j : pos x, [f;    pos2nat j##v] ~~> S (vec_pos w j))
-                               ->             [f;            x##v] ~~> 0
-                               ->             [ra_min f;        v] ~~> x
-where " [ f ; v ] ~~> x " := (@ra_bs _ f v x).
+    | in_ra_bs_c_min : forall min c k (f : recalg (S k)) v x w , x >= min ->
+                           (forall j : pos x, pos2nat j >= min -> [f;    pos2nat j##v; 0; c - (pos2nat j - min)] ~~> S (vec_pos w j)) 
+                                             ->             [f;            x##v; 0; c - (x - min)] ~~> 0
+                                             ->             [ra_min f;        v; min; S c] ~~> x
+where " [ f ; v ; min ; c ] ~~> x " := (@ra_bs_c min c _ f v x).
 
-
-Reserved Notation "  '[' f ';' v ';' c ']' '~~>' x " (at level 70).
-
-(* Bigstep semantics for recursive algorithms *)
-   
-Inductive ra_bs_c : nat -> forall k, recalg k -> vec nat k -> nat -> Prop := 
-    | in_ra_bs_c_cst  : forall c n v,             [ra_cst n;        v; S c] ~~> n
-    | in_ra_bs_c_zero : forall c v,               [ra_zero;         v; S c] ~~> 0
-    | in_ra_bs_c_succ : forall c v,               [ra_succ;         v; S c] ~~> S (vec_head v)
-    | in_ra_bs_c_proj : forall c k v j,           [@ra_proj k j;    v; S c] ~~> vec_pos v j 
-    
-    | in_ra_bs_c_comp : forall c k i f (gj : vec (recalg i) k) v w x,
-                                         (forall j, [vec_pos gj j;    v; c + k - pos2nat j] ~~> vec_pos w j)
-                                 ->             [f;               w; c] ~~> x
-                                 ->             [ra_comp f gj;    v; S c + 1 + k] ~~> x
-
-    | in_ra_bs_c_rec_0 : forall c k f (g : recalg (S (S k))) v x,    
-                                               [f;               v; c] ~~> x 
-                                 ->             [ra_rec f g;   0##v; S c] ~~> x
-
-    | in_ra_bs_c_rec_S : forall c k f (g : recalg (S (S k))) v n x y,          
-                                              [ra_rec f g;   n##v; c] ~~> x
-                               ->             [g;         n##x##v; c] ~~> y
-                               ->             [ra_rec f g; S n##v; S c] ~~> y
-                               
-    | in_ra_bs_c_min : forall c k (f : recalg (S k)) v x w , 
-                           (forall j : pos x, [f;    pos2nat j##v; c - pos2nat j] ~~> S (vec_pos w j)) 
-                               ->             [f;            x##v; c] ~~> 0
-                               ->             [ra_min f;        v; S c] ~~> x
-where " [ f ; v ; c ] ~~> x " := (@ra_bs_c c _ f v x).
-
-Lemma ra_bs_mono k (f : recalg k) v c1 x :
-  [f ; v ; c1 ] ~~> x -> forall c2, c1 <= c2 -> [f ; v ; c2] ~~> x. 
+Lemma ra_bs_mono min k (f : recalg k) v c1 x :
+  [f ; v ; min ; c1 ] ~~> x -> forall c2, c1 <= c2 -> [f ; v ; min; c2] ~~> x. 
 Proof.
   induction 1; intros; try (destruct c2;[ omega | ]).
   - econstructor.
   - econstructor.
   - econstructor.
   - econstructor.
-  - assert (S c2 = S (c2 - k - 1) + 1 + k ) as -> by omega.
-    econstructor.
+  - destruct c2; try omega. econstructor.
     + intros. eapply H0. omega.
     + eapply IHra_bs_c. omega.
   - econstructor. eapply IHra_bs_c. omega.
@@ -96,7 +50,8 @@ Proof.
     + eapply IHra_bs_c1. omega.
     + eapply IHra_bs_c2. omega.
   - econstructor.
-    + intros. eapply H0. omega.
+    + omega.
+    + intros. eapply H1. omega. omega.
     + eapply IHra_bs_c. omega.
 Qed.
 
@@ -111,8 +66,18 @@ Proof.
   - depelim j. omega. specialize (IHcst j). omega.
 Qed.
 
+Lemma ra_bs_from_c k (f : recalg k) c v x :
+ [f ; v ; 0 ; c] ~~> x -> [ f; v ] ~~> x.
+Proof.
+  remember 0 as min.
+  induction 1; subst; eauto using ra_bs.
+
+  econstructor. intros. eapply H1; omega.
+  eauto.
+Qed.
+
 Lemma ra_bs_to_c k (f : recalg k) v x :
-  [ f; v ] ~~> x -> exists c, [f ; v ; c ] ~~> x.
+  [ f; v ] ~~> x -> exists c, [f ; v ; 0 ; c] ~~> x.
 Proof.
   induction 1.
   - exists 1. econstructor.
@@ -121,7 +86,7 @@ Proof.
   - exists 1. econstructor.
   - destruct IHra_bs as [c].
     eapply vec_reif in H0 as [cst].
-    exists (1 + c + vec_sum cst + 1 + k). cbn.
+    exists (2 + c + vec_sum cst + k). cbn.
     econstructor.
     + intros. eapply ra_bs_mono. eauto.
       rewrite <- Nat.add_sub_assoc.
@@ -139,7 +104,7 @@ Proof.
   - destruct IHra_bs as [c].
     eapply vec_reif in H0 as [cst].
     exists (1 + c + vec_sum cst + x). cbn.
-    econstructor. 
+    econstructor. omega. 
     + intros. eapply ra_bs_mono. eauto.
       rewrite <- Nat.add_sub_assoc.
       2: pose (pos2nat_prop j); omega.
@@ -158,14 +123,6 @@ Inductive reccode :=
 | rc_nil
 | rc_rec (f : reccode) (g : reccode)
 | rc_min (f : reccode).
-
-Run TemplateProgram (tmGenEncode "enc_reccode" reccode).
-Hint Resolve enc_reccode_correct : Lrewrite.
-
-Instance term_rc_comp: computable rc_comp. extract constructor. Qed.
-Instance term_rc_cons : computable rc_cons.  extract constructor. Qed.
-Instance term_rc_rec : computable rc_rec.  extract constructor. Qed.
-Instance term_rc_min : computable rc_min.  extract constructor. Qed.
 
 Fixpoint eval (fuel : nat) (min : nat) (c : reccode) (v : list nat) : option (nat + list nat) :=
   match fuel with
@@ -205,66 +162,6 @@ Fixpoint eval (fuel : nat) (min : nat) (c : reccode) (v : list nat) : option (na
     end
   end.
 
-(* Lemma eval_mono_S fuel min c v r : *)
-(*   eval fuel min c v = Some r -> eval (S fuel) min c v = Some r. *)
-(* Proof. *)
-(*   intros. induction fuel in H, c, min, r, v |- *. *)
-(*   - inv H. *)
-(*   - cbn in H. destruct c; eauto. *)
-(*     + assert (IH2 := IHfuel min c2 v). *)
-(*       destruct (eval fuel min c2 v); try congruence. *)
-(*       destruct s; try congruence. *)
-(*       assert (IH1 := IHfuel min c1 l). *)
-(*       destruct (eval fuel min c1 l); try congruence. *)
-(*       specialize (IH1 _ eq_refl). specialize (IH2 _ eq_refl). *)
-(*       remember (S fuel) as n. cbn. *)
-(*       rewrite IH2, IH1. eassumption. *)
-(*     + assert (IH1 := IHfuel min c1 v). *)
-(*       destruct (eval fuel min c1 v); try congruence. *)
-(*       destruct s; try congruence. *)
-(*       assert (IH2 := IHfuel min c2 v). *)
-(*       destruct (eval fuel min c2 v); try congruence. *)
-(*       destruct s; try congruence. inv H. *)
-(*       specialize (IH1 _ eq_refl). specialize (IH2 _ eq_refl). *)
-(*       remember (S fuel) as k. cbn. *)
-(*       now rewrite IH2, IH1. *)
-(*     + *)
-(* Admitted. *)
-
-(* Lemma eval_mono fuel1 fuel2 min c v r : *)
-(*   eval fuel1 min c v = Some r -> fuel1 <= fuel2 -> eval fuel2 min c v = Some r. *)
-(* Proof. *)
-(*   intros. induction H0. *)
-(*   - eauto. *)
-(*   - eapply eval_mono_S. eauto. *)
-(* Qed. *)
-
-(* Inductive bigstep (min : nat) : reccode -> list nat -> nat -> Prop := *)
-(* | sem_cst v n : bigstep min (rc_cst n) v n *)
-(* | sem_zero v : bigstep min (rc_zero) v 0 *)
-(* | sem_succ x v : bigstep min (rc_succ) (x :: v) (S x) *)
-(* | sem_proj n v r : nth_error v n = Some r -> bigstep min (rc_proj n) v r *)
-(* | sem_comp f g G v r : bigstep_list min g v G -> bigstep min f G r -> bigstep min (rc_comp f g) v r *)
-(* | sem_rec1 f g v r : bigstep min f v r -> bigstep min (rc_rec f g) (0 :: v) r *)
-(* | sem_rec2 f g n v y x : bigstep min (rc_rec f g) (n :: v) y -> bigstep min g (n :: y :: v) x -> bigstep min (rc_rec f g) (S n :: v) x *)
-(* | sem_min f x v w : min <= x -> |w| >= x -> bigstep 0 f (x :: v) 0 -> (forall p n, min <= p < x -> nth_error w p = Some n -> bigstep 0 f (p :: v) (S n)) -> bigstep min (rc_min f) v x *)
-(* with bigstep_list (min : nat) : reccode -> list nat -> list nat -> Prop := *)
-(* | sem_cons f g v r G : bigstep min f v r -> bigstep_list min g v G -> bigstep_list min (rc_cons f g) v (r :: G) *)
-(* | sem_nil v : bigstep_list min (rc_nil) v nil. *)
-
-Inductive bigstep (min : nat) : nat -> reccode -> list nat -> nat -> Prop :=
-| sem_cst c v n : bigstep min (S c) (rc_cst n) v n
-| sem_zero c v : bigstep min (S c) (rc_zero) v 0
-| sem_succ c x v : bigstep min (S c) (rc_succ) (x :: v) (S x)
-| sem_proj c n v r : nth_error v n = Some r -> bigstep min (S c) (rc_proj n) v r
-| sem_comp c f g G v r : bigstep_list min c g v G -> bigstep min c f G r -> bigstep min (S c) (rc_comp f g) v r
-| sem_rec1 c f g v r : bigstep min c f v r -> bigstep min (S c) (rc_rec f g) (0 :: v) r
-| sem_rec2 c f g n v y x : bigstep min c (rc_rec f g) (n :: v) y -> bigstep min c g (n :: y :: v) x -> bigstep min (S c) (rc_rec f g) (S n :: v) x
-| sem_min c f x v w : min <= x -> |w| >= x -> bigstep 0 c f (x :: v) 0 -> (forall p n, min <= p < x -> nth_error w p = Some n -> bigstep 0 (c + x - p) f (p :: v) (S n)) -> bigstep min (c + x - min) (rc_min f) v x
-with bigstep_list (min : nat) : nat -> reccode -> list nat -> list nat -> Prop :=
-| sem_cons c f g v r G : bigstep min c f v r -> bigstep_list min c g v G -> bigstep_list min (S c) (rc_cons f g) v (r :: G)
-| sem_nil c v : bigstep_list min c (rc_nil) v nil.
-
 Definition rec_erase i (erase : forall i, recalg i -> reccode) := (fix rec k (v : vec (recalg i) k) := match v with vec_nil => rc_nil | vec_cons _ x v => rc_cons (erase _ x) (rec _ v) end).
 
 Fixpoint erase k (f : recalg k) : reccode :=
@@ -289,13 +186,65 @@ Proof.
     + eapply IHv.
 Qed.
 
-Lemma erase_correct k (f : recalg k) v n c  :
-  (ra_bs_c c f v n <-> eval c 0 (erase f) (vec_list v) = Some (inl n)).
-  (* (forall i (g : vec (recalg i) k) w v', (forall j : pos k, [vec_pos g j; v'; c - pos2nat j ] ~~> vec_pos w j) <-> eval c 0 (rec_erase erase g) (vec_list v') = Some (inr (vec_list w))). *)
+Lemma eval_inv n min i k (v : vec (recalg i) k) a l :
+  eval n min (rec_erase erase v) a = Some (inr l) ->
+  exists x, vec_list x = l /\
+  (forall j : pos k, eval (n -S (pos2nat j)) min (erase (vec_pos v j)) a = Some (inl (vec_pos x j))).
+Proof.
+  induction v in n,l |- *.
+  - destruct n; cbn. firstorder congruence. exact vec_nil. intros [=]. subst. exists vec_nil. split. reflexivity. intros. depelim j.
+  - destruct n. inversion 1.
+    intros ?. cbn in H.
+    destruct (eval n) eqn:E1; try congruence.
+    destruct s; try congruence.
+    destruct (eval n min (rec_erase erase v) a) eqn:E2; try congruence.
+    destruct s; try congruence. inv H. 
+    edestruct IHv as (? & ? & ?). eauto.
+    exists (vec_cons n1 x0). split. cbn. firstorder congruence.
+    intros j. depelim j.
+    + rewrite pos2nat_fst in *. assert (S n - 1 = n) by omega. rewrite H1 in *.
+      cbn -[eval].  eassumption.
+    + rewrite pos2nat_nxt.
+      specialize (H0 j). 
+      assert (S n - S (S (pos2nat j)) = n - S (pos2nat j)) by omega. rewrite H1 in *.
+      rewrite H0. reflexivity.
+Qed.
+
+Lemma le_ind2 m (P : nat -> Prop) :
+  P m -> (forall n, P (S n) -> S n <= m -> P n) -> forall n, n <= m -> P n.
+Proof.
+  intros. induction H1.
+  - eauto.
+  - eauto.
+Qed. 
+
+Lemma vec_pos_gt n X (w : vec X n) j k n1:
+  pos2nat k < pos2nat j ->
+  vec_pos w j = vec_pos (vec_change w k n1) j.
+Proof.
+  intros.
+  induction w.
+  - cbn. depelim j.
+  - cbn. depelim j.
+    + depelim k.
+      * cbn. omega.
+      * cbn. reflexivity.
+    + depelim k.
+      * cbn. reflexivity.
+      * cbn. eapply IHw. rewrite !pos2nat_nxt in *. omega.
+Qed.
+
+Lemma erase_correct k min (f : recalg k) v n c  :
+  (ra_bs_c min c f v n <-> eval c min (erase f) (vec_list v) = Some (inl n)).
 Proof.
   revert all except c.
   pattern c. eapply lt_wf_ind. intros.
   destruct f; cbn. 
+  - split.
+    + inversion 1. subst.
+      eapply EqDec.inj_right_pair in H4. subst.
+      reflexivity.
+    + destruct n; inversion 1. subst. econstructor.
   - split.
     + inversion 1. subst.
       eapply EqDec.inj_right_pair in H3. subst.
@@ -303,235 +252,186 @@ Proof.
     + destruct n; inversion 1. subst. econstructor.
   - split.
     + inversion 1. subst.
-      eapply EqDec.inj_right_pair in H2. subst.
-      reflexivity.
-    + destruct n; inversion 1. subst. econstructor.
-  - split.
-    + inversion 1. subst.
-      eapply EqDec.inj_right_pair in H2. subst.
+      eapply EqDec.inj_right_pair in H3. subst.
       cbn. depelim v. cbn. reflexivity.
     + destruct n; inversion 1. depelim v. subst. cbn in H2. inv H2. econstructor.
   - split.
     + inversion 1. subst.
-      eapply EqDec.inj_right_pair in H4. subst.
       eapply EqDec.inj_right_pair in H5. subst.
+      eapply EqDec.inj_right_pair in H6. subst.
       cbn. rewrite vec_list_nth. reflexivity.
     + destruct n; inversion 1. rewrite vec_list_nth in H2. inv H2. econstructor.
   - split.
     + inversion 1. subst.
       eapply EqDec.inj_right_pair in H2. subst.
       eapply EqDec.inj_right_pair in H7. subst.
-      eapply EqDec.inj_right_pair in H6. subst.
-      eapply EqDec.inj_right_pair in H6. subst.
-      assert (forall j : pos k, eval (c0 + k - pos2nat j) 0 (erase (vec_pos v0 j)) (vec_list v) = Some (inl (vec_pos w j))).
+      eapply EqDec.inj_right_pair in H7. subst.
+      eapply EqDec.inj_right_pair in H8. subst.
+      assert (forall j : pos k, eval (c0 - pos2nat j) min (erase (vec_pos v0 j)) (vec_list v) = Some (inl (vec_pos w j))).
       intros. eapply H. omega.
                                       
-      cbn. eapply H in H9. 2:omega. eauto.
-      eapply H in H9. 2:omega. cbn.
+      cbn. eapply H. omega. eapply H. omega. specialize (H9 j).
+      eapply H in H9. 2:omega. eapply H. omega. eauto.
+      remember (S c0) as c'. cbn.
 
-      assert (eval (c0 + 1 + k) 0 (rec_erase erase v0) (vec_list v) = Some (inr (vec_list w))).
-      { clear - H1. induction v0.
-        - cbn. assert (c0 + 1 + 0 = S c0) as -> by omega. cbn. depelim w. reflexivity.
-        - cbn. assert (c0 + 1 + S n = S c0 + 1 + n) as -> by omega.
-          cbn. pose proof (H1 pos_fst). cbn in H. rewrite pos2nat_fst in H.
-          assert (c0 + S n - 0 = c0 + 1 + n) by omega. rewrite H0 in *. clear H0.
-          rewrite H. depelim w. erewrite IHv0.  reflexivity.
+      assert (eval c' min (rec_erase erase v0) (vec_list v) = Some (inr (vec_list w))).
+      { subst. clear - H1. revert c0 H1. induction v0; intros.
+        - cbn. depelim w. reflexivity.
+        - cbn. pose proof (H1 pos_fst). cbn in H. rewrite pos2nat_fst in H.
+          replace (c0 - 0) with c0 in H by omega. rewrite H.
+          depelim w. destruct c0. cbn in H. inv H. erewrite IHv0.
+          reflexivity.
           intros. specialize (H1 (pos_nxt j)). rewrite pos2nat_nxt in H1.
-          assert (c0 + n - pos2nat j = c0 + S n - S (pos2nat j)) as -> by omega.
-          rewrite H1. reflexivity.
+          eassumption.
       }
-      rewrite H2. admit.
-    + 
-
-
-      edestruct H with (m := c0) as [_ ]. omega.
-      eapply H1 in H8. clear H1. rewrite H8, H9. reflexivity.
+      rewrite H2. subst. eapply H in H10. rewrite H10. reflexivity. omega.
     + destruct n; inversion 1.
-      destruct (eval n 0 (rec_erase erase v0) (vec_list v)) eqn:E; try congruence.
+      destruct (eval n min (rec_erase erase v0) (vec_list v)) eqn:E; try congruence.
       destruct s; try congruence.
-      destruct (eval n 0 (erase f) l) eqn:E2; try congruence.
-      destruct s; try congruence.
-      inv H2.
-      destruct (list_vec l). rewrite <- e in *. clear e.
-      econstructor.
-      * edestruct H with (m := n) as [_ ].
-        omega.
-        specialize (H1 i v0 x).
+      destruct (eval n min (erase f) l) eqn:E2; try congruence.
+      destruct s; try congruence. inv H2.
+      destruct n; try now inv E2.
 
-      * eapply H. omega. 
+      destruct (list_vec l). 
+      destruct (eval_inv E) as (w & ? & ?). subst.
 
-
-Lemma erase_correct k (f : recalg k) v n c :
-  ra_bs_c c f v n <-> bigstep 0 c (erase f) (vec_list v) n.
-Proof.
-  revert k f v n.
-  pattern c. eapply lt_wf_ind. intros.
-  destruct f.
-  - split; inversion 1; econstructor.
-  - split; inversion 1; econstructor.
-  - split.
-    + intros. inversion H0. subst.
-      eapply EqDec.inj_right_pair in H2. subst.
-      depelim v. econstructor.
-    + intros. inversion H0. subst.
-      depelim v. cbn in H2. inv H2. econstructor.
-  - split.
-    + intros. inversion H0. subst.
-      eapply EqDec.inj_right_pair in H4. subst.
+      eapply in_ra_bs_c_comp with (w := w).
+      * intros. eapply H. omega. specialize (H2 j). assert (S n - S (pos2nat j) = n - pos2nat j) by omega. rewrite H1 in *.
+        eauto.
+      * eapply H. omega. eassumption.
+  - split. inversion 1.
+    + eapply EqDec.inj_right_pair in H4. subst.
+      eapply EqDec.inj_right_pair in H6. subst.
+      eapply EqDec.inj_right_pair in H7. subst.
+      cbn.
+      eapply H in H8. 2:omega. rewrite H8. reflexivity.
+    + eapply EqDec.inj_right_pair in H2. subst.
       eapply EqDec.inj_right_pair in H5. subst.
-      econstructor. clear. eapply vec_list_nth.              
-    + intros. inversion H0. subst.
-      rewrite vec_list_nth in H3. inv H3. econstructor.
+      eapply EqDec.inj_right_pair in H6. subst.
+      eapply H in H7.
+      cbn. 2:omega. rewrite H7.
+      eapply H in H9. 2:omega. rewrite H9. reflexivity.
+    + intros. destruct n; inv H0.
+      depelim v. cbn in H2. destruct n1.
+      * destruct (eval n min (erase f1) (vec_list v)) eqn:E.
+        destruct s; inv H2.
+        -- econstructor. eapply H. omega. eauto.
+        -- econstructor. congruence.
+      * destruct eval eqn:E2; try congruence.
+        destruct s; try congruence.
+        destruct (eval n min (erase f2)) eqn:E3.
+        destruct s; inv H2.
+        -- econstructor. eapply H. omega. eauto. eapply H. omega. eauto.
+        -- congruence.
   - split.
-    + intros. cbn.
-      admit.
-    + admit.
-  - split.
-    + intros. inversion H0. subst.
-      * eapply EqDec.inj_right_pair in H3. subst.
-        eapply EqDec.inj_right_pair in H5. subst.
-        eapply EqDec.inj_right_pair in H6. subst.
-        cbn. econstructor. eapply H. omega. eauto.
-      * eapply EqDec.inj_right_pair in H2. subst.
-        eapply EqDec.inj_right_pair in H5. subst.
-        eapply EqDec.inj_right_pair in H4. subst.
-        cbn. econstructor.
-        -- eapply H with (f := ra_rec f1 f2) (v := vec_cons n1 v0). omega. eauto. 
-        -- eapply H with (v := vec_cons n1 (vec_cons x v0)). omega. eauto. 
-    + intros. inversion H0; subst.
-      * depelim v. inv H5. econstructor. eapply H. omega. eauto.
-      * depelim v. inv H4. econstructor. eapply H. omega. eauto.
-        eapply H. omega. eauto.
-  - split.
-    + 
+    + inversion 1. subst.
+      eapply EqDec.inj_right_pair in H1. subst.
+      eapply EqDec.inj_right_pair in H2. subst.
+      clear H0. unfold ge in *.
+      revert c0 H w H7 H8. pattern n0. revert min H3.
+      eapply le_ind2; intros.
+      * cbn in *. eapply H in H8. 2:omega.
+        assert (c0 - (n0 - n0) = c0) by lia. rewrite H0 in *.
+        rewrite H8. reflexivity.
+      * destruct n0; try omega.
+        assert (n < S n0) by omega.
+        assert (H10 := H7).
+        specialize (H7 (nat2pos H2)). rewrite pos2nat_nat2pos in H7.
+        assert (n <= n) by omega. eapply H7 in H3.
+        eapply H1 in H3. 2: omega. cbn.
+        assert (c0 - (n - n) = c0) by omega. rewrite H4 in *. rewrite H3.
 
+        assert (eval c0 (S n) (rc_min (erase f)) (vec_list v) = Some (inl (S n0))).
+        eapply H1 with (f := ra_min f). omega.
 
-  split.
-  - intros. induction H.
-    + econstructor.
-    + econstructor.
-    + depelim v. depelim v. cbn. econstructor.
-    + econstructor.      
-      depind v; cbn.
-      * depelim j.
-      * depelim j.
-        -- rewrite pos2nat_fst. reflexivity.
-        -- rewrite pos2nat_nxt. cbn. eauto.
-    + admit.
-    + econstructor. eauto.
-    + econstructor. eauto. eauto.
-    + eapply sem_min with (w := vec_list w).
-      * omega.
-      * rewrite vec_list_length. omega.
-      * eauto. 
-      * intros. admit.
-  - 
+        destruct c0. inv H3.
+        econstructor. omega.
+           
+        intros ? ?. specialize (H10 j).
+        assert (S c0 - (pos2nat j - n) = c0 - (pos2nat j - S n)) by omega.
+        rewrite H6 in *.  eapply H10. omega.
+        assert (S c0 - (S n0 - n) = c0 - (S n0 - S n)) by lia. rewrite H5 in *.
+        eassumption.
+        now rewrite H5.
+    + intros.
+      destruct n; try now inv H0. cbn in H0.
+      destruct (eval n) eqn:E1; try now inv H0.
+      destruct s; try congruence.
+      destruct n1; inv H0.
+      * econstructor. omega. intros. pose proof (pos2nat_prop j). omega.
+        eapply H. omega. assert (n - (n0 - n0) = n) as -> by omega. eassumption.
+      * destruct (eval n (S min)) eqn:E2; try now inv H2.
+        destruct s; inv H2.
+        eapply H with (f := ra_min f) in E2. 2:omega.
+        eapply H with (v := vec_cons min v) in E1. 2:omega.
+        inversion E2; subst.
+        eapply EqDec.inj_right_pair in H0. subst.
+        eapply EqDec.inj_right_pair in H1. subst.
+        assert (min < n0) by omega.
+        eapply in_ra_bs_c_min with (w := vec_change w (nat2pos H0) n1).
+        -- omega.
+        -- intros. inversion H1.
+           ++ subst.
+              rewrite nat2pos_pos2nat.
+              rewrite vec_change_eq. 2:reflexivity.
+              assert (S c0 - (pos2nat j - pos2nat j) = S c0) as -> by omega.
+              eassumption.
+           ++ specialize (H6 j).
+              assert (S c0 - (S m - min) = c0 - (pos2nat j - S min)) by lia. rewrite H5 in *.
+              enough (vec_pos w j = vec_pos (vec_change w (nat2pos H0) n1) j).
+              rewrite H8 in H6. rewrite H3. eapply H6. omega.
+              assert (pos2nat j > min) by omega.
+              eapply vec_pos_gt.
+              rewrite pos2nat_nat2pos. omega.
+        -- assert (S c0 - (n0 - min) = c0 - (n0 - S min)) by omega. rewrite H1. eassumption.
+           Grab Existential Variables. exact vec_zero.
+Qed.
 
+Run TemplateProgram (tmGenEncode "enc_reccode" reccode).
+Hint Resolve enc_reccode_correct : Lrewrite.
 
-Import ListNotations.
-
-Fixpoint update X (l : list X) n x :=
-  match n, l with
-  | 0, _ :: l => x :: l
-  | S n, y :: l => y :: update l n x
-  | _, [] => []
-  end.
-
-Lemma eval_bigstep fuel min c v r :
-  eval fuel min c v = Some r ->
-  match r with
-  | inl n => bigstep min fuel c v n
-  | inr L => bigstep_list min fuel c v L
-  end.
-Proof.
-  revert min c v r. induction fuel; cbn; intros; try destruct c; try congruence.
-  all: try now (inv H; econstructor).
-  - destruct v; inv H. econstructor.
-  - destruct (nth_error v n) eqn:E; inv H. now econstructor.
-  - assert (IH2 := IHfuel min c2 v).
-    destruct (eval fuel min c2 v). destruct s. all:try congruence.
-    assert (IH1 := IHfuel min c1 l).
-    destruct (eval fuel min c1 l). destruct s. all:try congruence.
-    specialize (IH1 _ eq_refl). specialize (IH2 _ eq_refl). inv H. cbn in *.
-    econstructor. eauto. eauto.
-  - assert (IH1 := IHfuel min c1 v).
-    destruct (eval fuel min c1 v). destruct s. all:try congruence.
-    assert (IH2 := IHfuel min c2 v).
-    destruct (eval fuel min c2 v). destruct s. all:try congruence.
-    specialize (IH1 _ eq_refl). specialize (IH2 _ eq_refl). inv H. cbn in *.
-    econstructor. eauto. eauto.
-  - destruct v; try congruence.
-    destruct n.
-    + assert (IH1 := IHfuel min c1 v).
-      destruct (eval fuel min c1 v). destruct s. all:try congruence. inv H.
-      specialize (IH1 _ eq_refl). cbn in *.
-      econstructor. eauto.
-    + assert (IH2 := IHfuel min (rc_rec c1 c2) (n :: v)).
-      destruct (eval fuel min (rc_rec c1 c2) (n :: v)). destruct s. all:try congruence.
-      specialize (IH2 _ eq_refl).
-      assert (IH3 := IHfuel min c2 (n :: n0 :: v)).
-      destruct (eval fuel min c2 (n :: n0 :: v)). destruct s. all:try congruence. 
-      specialize (IH3 _ eq_refl). cbn in *. inv H.
-      econstructor. eauto. eauto.
-  - assert (IH1 := IHfuel 0 c (min :: v)).
-    destruct (eval fuel 0 c (min :: v)); try congruence.
-    destruct s; try congruence.
-    specialize (IH1 _ eq_refl).
-    destruct n.
-    + inv H. cbn in *. eapply sem_min with (w := repeat min min). eauto. eauto.
-      rewrite repeat_length. omega. eauto.
-      intros. omega. 
-    + assert (IH2 := IHfuel (S min) (rc_min c) v).
-      destruct (eval fuel (S min) (rc_min c) v); try congruence.
-      destruct s; inv H.
-      specialize (IH2 _ eq_refl). cbn in *. inversion IH2. subst.
-      eapply sem_min with (w := update w min n).
-      omega. admit. eauto. intros.
-      decide (min = p).
-      * subst. admit.
-      * eapply H3. omega. admit.
-Admitted.
-
-Scheme bigstep1_ind := Induction for bigstep Sort Prop
-  with bigstep2_ind := Induction for bigstep_list Sort Prop.
-Combined Scheme bigstepInd from bigstep1_ind, bigstep2_ind.
-
-Lemma bigstep_eval min  :
-  (forall c v n, bigstep min c v n -> exists fuel, eval fuel min c v = Some (inl n)) /\
-  (forall c v L, bigstep_list min c v L -> exists fuel, eval fuel min c v = Some (inr L)).
-Proof.
-  apply bigstepInd with (P := fun min c v n _ => exists fuel : nat, eval fuel min c v = Some (inl n)) (P0 := fun min c v L _ => exists fuel : nat, eval fuel min c v = Some (inr L)).
-  all: cbn; intros.
-  all: try now exists 1; eauto.
-  - exists 1. cbn. now rewrite e. 
-  - destruct H, H0.
-    exists (1 + x + x0). 
-    cbn. erewrite eval_mono; eauto.
-    cbn. erewrite eval_mono; eauto.
-    eauto. omega. omega.
-  - destruct H.
-    exists (1 + x). 
-    cbn. erewrite eval_mono; eauto.
-    eauto.
-  - destruct H, H0.
-    exists (1 + x0 + x1). 
-    cbn. erewrite eval_mono; eauto.
-    cbn. erewrite eval_mono; eauto.
-    eauto. omega. omega.
-  - destruct H.
-    exists (1 + x0). 
-    cbn. decide (min0 = x).
-    + subst. now rewrite H.
-    + assert (min0 <= min0 < x). omega. eapply H0 in H1 as [].
-      admit. admit.
-  - destruct H, H0.
-    exists (1 + x0 + x). 
-    cbn. erewrite eval_mono; eauto.
-    cbn. erewrite eval_mono; eauto.
-    eauto. omega. omega.
-Admitted.
+Instance term_rc_comp: computable rc_comp. extract constructor. Qed.
+Instance term_rc_cons : computable rc_cons.  extract constructor. Qed.
+Instance term_rc_rec : computable rc_rec.  extract constructor. Qed.
+Instance term_rc_min : computable rc_min.  extract constructor. Qed.
 
 Instance term_eval : computable eval.
 Proof.
   extract.
 Qed.
+
+Definition evalfun fuel c v := match eval fuel 0 c v with Some (inl x) => Some x | _ => None end.
+
+Definition UMUREC_HALTING c := exists fuel, evalfun fuel c nil <> None.
+
+From Undecidability.Problems Require Import Reduction.
+
+Lemma MUREC_red : MUREC_HALTING ⪯ UMUREC_HALTING.
+Proof.
+  unshelve eexists.
+  - intros f. exact (erase f).
+  - unfold UMUREC_HALTING, MUREC_HALTING. 
+    intros f.
+    split; intros [].
+    + rewrite ra_bs_correct in H. eapply ra_bs_to_c in H as [].
+      exists x0. eapply erase_correct in H. unfold evalfun. rewrite H. congruence.
+    + unfold evalfun in H. destruct eval eqn:E; try congruence.
+      destruct s; try congruence.
+      eapply erase_correct with (v := vec_nil) in E.
+      exists n. eapply ra_bs_correct. now eapply ra_bs_from_c.
+Qed.
+
+Local Definition r := (fun c n => match eval n 0 c [] with Some (inl n) => true | _ => false end).
+
+Lemma MUREC_WCBV : MUREC_HALTING ⪯ converges.
+Proof.
+  eapply reduces_transitive. eapply MUREC_red.
+  eapply L_recognisable_halt.
+  exists (fun c n => match eval n 0 c [] with Some (inl n) => true | _ => false end).
+  split.
+  - econstructor. extract.
+  - firstorder.
+    + unfold evalfun in *. exists x0. destruct eval; try destruct s; try congruence.
+    + exists x0. unfold evalfun in *. destruct eval; try destruct s; try congruence.
+Qed.
+Print Assumptions MUREC_WCBV.
